examples/algorithms/downgrade.fst
@@ -1,5 +1,5 @@
 module Downgrade
-
+#set-options "--initial_fuel 0 --initial_ifuel 0 --max_fuel 0 --max_ifuel 0"
 open Array
 open Seq
 open SeqProperties
@@ -12,7 +12,6 @@ assume val qsort_arr: a:Type -> f:tot_ord a -> x:array a -> ST unit
   (ensures (fun h0 u h1 -> contains h1 x /\ sorted f (sel h1 x) /\ permutation a (sel h0 x) (sel h1 x)))
   (modifies (a_ref x))
 
-
 val qsort_seq : a:Type -> f:tot_ord a -> x:seq a -> ST (seq a)
   (requires (fun h -> True))
   (ensures (fun h0 y h1 -> sorted f y /\ permutation a x y))
@@ -24,25 +23,24 @@ let qsort_seq f x =
   free x_ar;
   res
 
-(* #reset-options *)
-(* assume val down: a:Type -> b:(a -> Type) -> req:(a -> heap -> Type) -> ens:(x:a -> heap -> b x -> heap -> Type)  *)
-(*          -> =f:(x:a -> ST (b x) (req x) (ens x) no_refs){(forall (x:a) (h:heap). req x h)} *)
-(*          -> Tot (x:a -> Div (b x) True (fun (y:b x) -> exists h0 h1. ens x h0 y h1)) *)
+assume val down: a:Type -> b:(a -> Type) -> req:(a -> heap -> Type) -> ens:(x:a -> heap -> b x -> heap -> Type)
+         -> =f:(x:a -> ST (b x) (req x) (ens x) no_refs){(forall (x:a) (h:heap). req x h)}
+         -> Tot (x:a -> Div (b x) True (fun (y:b x) -> exists h0 h1. ens x h0 y h1))
 
-(* val qsort_seq_down: a:Type -> f:tot_ord a -> s1:seq a -> Dv (s2:seq a{sorted f s2 /\ permutation a s1 s2}) *)
-(* let qsort_seq_down f x = down (qsort_seq f)  x *)
-
-
-(* assume val forget_ST: #a:Type -> #b:(a -> Type)  *)
-(*   -> #req:(a -> heap -> Type)  *)
-(*   -> #ens:(x:a -> heap -> b x -> heap -> Type)  *)
-(*   -> =f:(x:a -> ST (b x) (req x) (ens x) no_refs) *)
-(*      {forall x h h'. req x h ==> req x h'}  *)
-(*   -> Tot (x:a -> Div (b x)  *)
-(*                  (requires (forall h. req x h)) *)
-(*                  (ensures (fun (y:b x) -> exists h0 h1. ens x h0 y h1))) *)
+val qsort_seq_down: a:Type -> f:tot_ord a -> s1:seq a -> Dv (s2:seq a{sorted f s2 /\ permutation a s1 s2})
+let qsort_seq_down f x = down (qsort_seq f)  x
 
 
+assume val forget_ST: #a:Type -> #b:(a -> Type)
+  -> #req:(a -> heap -> Type)
+  -> #ens:(x:a -> heap -> b x -> heap -> Type)
+  -> =f:(x:a -> ST (b x) (req x) (ens x) no_refs)
+     {forall x h h'. req x h ==> req x h'}
+  -> Tot (x:a -> Div (b x)
+                 (requires (forall h. req x h))
+                 (ensures (fun (y:b x) -> exists h0 h1. ens x h0 y h1)))
 
-(* val qsort_seq_forget: a:Type -> f:tot_ord a -> s1:seq a -> Dv (s2:seq a{sorted f s2 /\ permutation a s1 s2}) *)
-(* let qsort_seq_forget f x = forget_ST (qsort_seq f)  x *)
+
+
+val qsort_seq_forget: a:Type -> f:tot_ord a -> s1:seq a -> Dv (s2:seq a{sorted f s2 /\ permutation a s1 s2})
+let qsort_seq_forget f x = forget_ST (qsort_seq f)  x
