examples/algorithms/qsort_arr.fst
@@ -1,22 +1,17 @@
-module QuickSort.Seq
+module QuickSort.Array
 open Array
 open Seq
+open SeqProperties
 open Heap
 open ST
-open SeqProperties
-open SeqPermutation
+#set-options "--initial_fuel 1 --initial_ifuel 0 --max_fuel 1 --max_ifuel 0 --admit_smt_queries false"
+type tot_ord (a:Type) = f:(a -> a -> Tot bool){total_order a f}
 
-(* (\* Defining a new predicate symbol *\) *)
-(* type total_order (a:Type) (f: (a -> a -> Tot bool)) = *)
-(*     (forall a. f a a)                                           (\* reflexivity   *\) *)
-(*     /\ (forall a1 a2. (f a1 a2 /\ a1<>a2)  <==> not (f a2 a1))  (\* anti-symmetry *\) *)
-(*     /\ (forall a1 a2 a3. f a1 a2 /\ f a2 a3 ==> f a1 a3)        (\* transitivity  *\) *)
+(* replaces the [i,j) sub-sequence of s1 with the corresponding sub-sequence of s2 *)
+let splice (a:Type) (s1:seq a) (i:nat) (s2:seq a{length s1=length s2})  (j:nat{i <= j /\ j <= (length s2)})
+    = Seq.append (slice s1 0 i) (Seq.append (slice s2 i j) (slice s1 j (length s1)))
 
-let splice (a:Type) (s1:seq a) (i:nat) (s2:seq a{s1.length=s2.length})  (j:nat{i <= j /\ j <= s2.length})
-    = Seq.append (slice s1 0 i) (Seq.append (slice s2 i j) (slice s1 j s1.length))
-
-
-assume val partition: a:Type -> f:(a -> a -> Tot bool){total_order a f} 
+assume val partition: a:Type -> f:tot_ord a
                -> start:nat -> len:nat{start <= len} 
                -> pivot:nat{start <= pivot /\ pivot < len} 
                -> back:nat{pivot <= back /\ back < len}
@@ -35,7 +30,7 @@ assume val partition: a:Type -> f:(a -> a -> Tot bool){total_order a f}
     /\ (length (sel h1 x) = length (sel h0 x))
     /\ (sel h1 x = splice (sel h0 x) start (sel h1 x) len)
     /\ ((fun orig lo hi p -> 
-               (hi.length > 0)
+               ((length hi) > 0)
             /\ (forall y. (mem y hi ==> f p y)
                        /\ (mem y lo ==> f y p)
                        /\ (count y orig = count y hi + count y lo)))
@@ -45,87 +40,89 @@ assume val partition: a:Type -> f:(a -> a -> Tot bool){total_order a f}
         (index (sel h1 x) i))))
   (modifies (a_ref x))
 
+(* assume val lemma_slice_splice: a:Type -> s1:seq a  *)
+(*          -> i:nat -> s2:seq a{length s2 = length s1} -> j:nat{i <= j /\ j <= (length s1)}  *)
+(*          -> k:nat{k <= i} -> Lemma *)
+(*   (requires True) *)
+(*   (ensures (slice (splice s1 i s2 j) k i = slice s1 k i)) *)
+(*   (\* [SMTPat (slice (splice s1 i s2 j) k i)] *\) *)
 
-assume val lemma_slice_splice: a:Type -> s1:seq a 
-         -> i:nat -> s2:seq a{length s2 = length s1} -> j:nat{i <= j /\ j <= s1.length} 
-         -> k:nat{k <= i} -> Lemma
-  (ensures (slice (splice s1 i s2 j) k i = slice s1 k i))
+(* assume val lemma_splice_append: a:Type -> s1:seq a -> i:nat -> s2:seq a{(length s1) = (length s2)} -> j:nat{i <= j /\ j<=(length s1)} *)
+(*          -> k:nat{k <= i} -> Lemma  *)
+(*          (requires True) *)
+(*          (ensures (slice (splice s1 i s2 j) k j = append (slice s1 k i) (slice s2 i j))) *)
+(*          (\* [SMTPat (slice (splice s1 i s2 j) k j)] *\) *)
 
-assume val lemma_splice_append: a:Type -> s1:seq a -> i:nat -> s2:seq a{s1.length = s2.length} -> j:nat{i <= j /\ j<=s1.length}
-         -> k:nat{k <= i} -> Lemma 
-         (ensures (slice (splice s1 i s2 j) k j = append (slice s1 k i) (slice s2 i j)))
+(* assume val lemma_slice_splice_append_cons: a:Type -> s1:seq a{(length s1) > 0} -> i:nat ->  p:nat{i < p} -> s2:seq a{(length s1) = (length s2)} -> j:nat{p <= j /\ j <= (length s1)} -> Lemma *)
+(*          (requires True)                                                                                                                                                                                   *)
+(*          (ensures (slice (splice s2 p s1 j) i j =  *)
+(*              append (slice s2 i (p - 1)) (cons (index s2 (p - 1)) (slice s1 p j)))) *)
+(*          (\* [SMTPat (slice (splice s2 p s1 j) i j)] *\) *)
 
-assume val lemma_slice_splice_append_cons: a:Type -> s1:seq a{s1.length > 0} -> i:nat ->  p:nat{i < p} -> s2:seq a{s1.length = s2.length} -> j:nat{p <= j /\ j <= s1.length} -> Lemma
-         (ensures (slice (splice s2 p s1 j) i j = 
-             append (slice s2 i (p - 1)) (cons (index s2 (p - 1)) (slice s1 p j))))
-
-val sort: a:Type -> f:(a -> a -> Tot bool){total_order a f} -> i:nat -> j:nat{i <= j} 
-          -> x:array a -> ST unit 
+assume val lemma_slice_mem: a:Type -> s:seq a -> i:nat -> j:nat{i <= j /\ j < length s} -> Lemma
+                           (requires True)
+                           (ensures (forall x. mem x (slice s i j) ==> mem x s))
+val sort: a:Type -> f:tot_ord a -> i:nat -> j:nat{i <= j} -> x:array a 
+          -> ST unit 
   (requires (fun h -> contains h x /\ j <= length (sel h x)))
-  (ensures (fun h0 u h1 -> (j <= length (sel h0 x)
-                            /\ contains h1 x
-                            /\ (length (sel h0 x) = length (sel h1 x))
-                            /\ sorted f (slice (sel h1 x) i j)
-                            /\ (sel h1 x = splice (sel h0 x) i (sel h1 x) j)
-                            /\ permutation a (slice (sel h0 x) i j) (slice (sel h1 x) i j))))
+  (ensures (fun h0 u h1 -> (j <= length (sel h0 x)                                      (* carrying this along from the requires clause *)
+                            /\ contains h1 x                                            (* the array is still in the heap *)
+                            /\ (length (sel h0 x) = length (sel h1 x))                  (* it's length has not changed *)
+                            /\ sorted f (slice (sel h1 x) i j)                          (* it is sorted between [i, j) *)
+                            /\ Eq (sel h1 x) (splice (sel h0 x) i (sel h1 x) j)         (* the rest of it is unchanged *)
+                            /\ permutation a (slice (sel h0 x) i j) (slice (sel h1 x) i j)))) (* the [i,j) sub-array is permutation of the original one *)
   (modifies (a_ref x))
-let rec sort f i j x = 
+let rec sort (a:Type) f i j x = 
   let h0 = ST.get () in
   if i=j 
-  then cut (Eq (sel h0 x) (splice (sel h0 x) i (sel h0 x) j))
-  else 
-    let pivot = partition f i j i (j - 1) x in
-    (* assert (pivot + 1 <= j); *)
-
-    let _h1 = ST.get () in
-    let lo = slice (sel _h1 x) i pivot in
-    let hi = slice (sel _h1 x) pivot j in
-    let p = index (sel _h1 x) pivot in
-    let hi_tl = tail hi in 
-    (* assert (sel h1 x = splice (sel h0 x) i (sel h1 x) j); *)
-    
-    sort f i pivot x;
-
-    let _h2 = ST.get () in    
-    let l = slice (sel _h2 x) i pivot in 
-    (* assert (sel _h2 x = splice (sel _h1 x) i (sel _h2 x) pivot); *)
-    (* assert (sorted f l); *)
-    (* let q = index (sel _h2 x) pivot in *)
-    (* cut (b2t (p=q)); *)
+  then ()
+  else begin
+      let h0 = get() in
+      let pivot = partition f i j i (j - 1) x in
+      
+      
+      let h1 = get() in
+      let pv = index (sel h1 x) pivot in
 
 
-    sort f (pivot + 1) j x;
+      sort f i pivot x;
+      let h2 = get() in
 
-    let _h3 = ST.get () in
-    let h = slice (sel _h3 x) (pivot + 1) j in
-    
-    (* assert (sel _h3 x = splice (sel _h2 x) (pivot + 1) (sel _h3 x) j); *)
-    (* assert (sorted f h); *)
+      cut (Eq (slice (sel h2 x) pivot j) (slice (sel h1 x) pivot j));
+      cut (Eq (tail (slice (sel h2 x) pivot j))
+              (slice (sel h2 x) (pivot + 1) j));
+      cut (forall y. mem y (slice (sel h2 x) (pivot + 1) j) ==> f pv y);
 
-    lemma_slice_splice (sel _h2 x) (pivot + 1) (sel _h3 x) j i;
-    assert (l=slice (sel _h3 x) i pivot);
-    
-    (* assert (j <= length (sel h2 x)); *)
-    let r = index (sel _h3 x) pivot in
-    (* assert (p = r); *)
+      sort f (pivot + 1) j x;
+      let h3 = get() in
 
-    lemma_slice_splice_append_cons (sel _h2 x) i (pivot + 1) (sel _h3 x) j;
+      (* assert (permutation a (slice (sel h2 x) (pivot + 1) j) *)
+      (*                       (slice (sel h3 x) (pivot + 1) j)); *)
+      cut (Eq (slice (sel h3 x) i pivot) (slice (sel h2 x) i pivot));
 
-    assert (slice (sel _h3 x) i j 
-            = (append l (cons (index (sel _h2 x) pivot) h)));
+      
+      (* cut (Eq (tail (slice (sel h3 x) pivot j)) (slice (sel h3 x) (pivot + 1) j)); *)
 
-    (* assert (p = index (sel _h2 x) pivot); *)
+      cut (forall y. mem y (slice (sel h3 x) i pivot) ==> f y pv);
+      cut (forall y. mem y (slice (sel h3 x) (pivot + 1) j) ==> f pv y);
 
-    (* assert (forall y. mem y l ==> f y p); *)
-    (* assert (forall y. mem y h ==> f p y); *)
-    (* sorted_concat_lemma f l p h; *)
-    (* assert (sorted f (append l (cons p h))); *)
 
-    (* lemma_append_count l (cons p h); *)
+      let lo = slice (sel h3 x) i pivot in
+      let hi = tail (slice (sel h3 x) pivot j) in
 
-    (* cons_perm h hi; *)
+      (* cut (sorted f lo); *)
+      (* cut (sorted f hi); *)
 
-    admit ()
+      (* cut (forall y. mem y lo ==> f y pv); *)
+
+      (* cut (forall y. mem y (slice (sel h3 x) pivot j) ==> f pv y); *)
+      (* SeqProperties.sorted_concat_lemma f lo pv hi; *)
+
+      (* cut (Eq (slice (sel h3 x) i j) (append lo (cons pv hi))); *)
+      (* assert (sorted f (slice (sel h3 x) i j)); *)
+      admit()
+
+    end
        
 
 (* val qsort: a:Type -> f:(a -> a -> Tot bool){total_order a f} -> x:array a -> ST unit  *)
